---
layout: post
title: Example of Latex on Blog
---

**Assignment:**\
\
**Problem I:** Let $E \subset {\mathbb{R}}$ be a non-empty set of real
numbers which is bounded above. When $a > 0$ is a positive real number,
let us set $$aE = \{ax; x \in E \}.$$ Prove that the set $aE$ is bounded
above and that $$\sup aE = a \sup E.$$ Solve the following exercises
from Ross: 3.5, 3.6, 4.1 (right hand column only, i.e. b, d, f, h, j, l,
n, p, r, t, v), 4.6, 4.7, 4.8, 4.10, 4.11, 4.12, 4.14, 4.15, 5.2.

#### Problem I:

Let $E \subset {\mathbb{R}}$ be a non-empty set of real numbers which is
bounded above. When $a > 0$ is a positive real number, let us set
$$aE = \{ax; x \in E \}.$$ Prove that the set $aE$ is bounded above and
that $$\sup aE = a \sup E.$$

Let $E \subset {\mathbb{R}}$ be a non-empty set of real numbers which is
bounded above. When $a > 0$ is a positive real number, let us set
$$aE = \{ax; x \in E \}.$$ Since $E$ is bounded above, there exists a
least upper bound of $E$ such that $x \leq \sup E$ $\forall x \in E$. By
multiplying $a$ to both sides of the inequality, $ax \leq a\sup E$
$\forall x \in E$. Therefore, $a \sup E$ is the upper bound of $aE$,
which implies that $aE$ is bounded above. With $\sup aE$ being the least
upper bound of $aE$, the upper bound $a \sup E$ must be greater than or
equal to $\sup aE$. Hence, $$\sup aE \leq a\sup E.$$ Given that $aE$ is
bounded above, there exists a least upper bound for $aE$ where
$ax \leq \sup aE$ $\forall ax \in aE$. If we algebraically manipulate
the inequality, $$ax \leq \sup aE$$
$$x \leq \frac{\sup aE}{a} \quad \forall x \in E,$$ which means that
$\frac{\sup aE}{a}$ is the upper bound of $E$. With $\sup E$ being the
least upper bound of $E$, $$\sup E \leq \frac{\sup aE}{a}.$$ Therefore,
if we multiply $a$ to both sides of the inequality,
$$a \sup E \leq \sup aE.$$ Since $\sup aE \leq a\sup E$ and
$a\sup E \leq \sup aE$, $$\sup aE = a\sup E.$$

#### 3.5

1.  Show $|b| \leq a$ if and only if $-a \leq b \leq a$.

    ($\implies$) Assume $|b| \leq a$. Then $-a \leq -|b|$ by property
    (i) of Theorem 3.2 from page 16 of Ross’ *Elementary Analysis* (2nd
    ed.), which states that

    *if $a \leq b$, then $-b \leq -a$.*

    By Definition 3.3 from page 17 of Ross’ *Elementary Analysis* (2nd
    ed.), which is the definition of absolute value,
    $-a \leq -|b| \leq b \leq |b| \leq a$. Thus, by transitivity,
    $-a \leq b \leq a$.\
    ($\impliedby$) Assume $-a \leq b \leq a$.

    -   If $b \geq 0$, $|b| = b \leq a$. Thus, $|b| \leq a$ by
        transitivity.

    -   If $b < 0$, $|b| = -b \leq a$ since $a \geq -b \geq -a$ by
        property (i) of Theorem 3.2. Thus, by transitivity,
        $|b| \leq a$.

    Therefore, $|b| \leq a$ if and only if $-a \leq b \leq a$.

2.  Prove $\|a\| - \|b\| \leq |a-b|$ for all $a,b \in {\mathbb{R}}$.

    Let $a,b \in {\mathbb{R}}$. By the associative and commutative
    property of real numbers,
    $$|a| = |a + (b-b) | = |a+b-b| = |a-b+b| = |(a-b) + b|$$ By the
    Triangle Inequality, we know that $$|(a-b) + b| \leq |a-b| + |b|.$$
    Thus, $|a| \leq |a-b| + |b|$, and if we subtract $|b|$ to both sides
    of the inequality, $$\|a\| - \|b\| \leq |a-b|.$$

#### 3.6

1.  Prove $|a+b+c| \leq |a| + |b| + |c|$ for all
    $a,b,c \in {\mathbb{R}}$. *Hint:* Apply the triangle inequality
    twice. Do *not* consider eight cases.

    Let $a,b,c \in {\mathbb{R}}$. By Triangle Inequality,
    $|a+b+c| = |(a+b)+c| \leq |a+b| + |c| \leq |a| + |b| + |c|$. Thus,
    by transitivity, $|a+b+c| \leq |a|+|b|+|c|$.

2.  Use induction to prove
    $$|a_1+a_2+\cdots+a_n| \leq |a_1| + |a_2| + \cdots + |a_n|$$ for $n$
    numbers $a_1,a_2,\ldots,a_n$.\
    \
    *Proof by Induction.* Given $n \in {\mathbb{N}}$, our $n$th
    proposition is
    $$P_n : ``|a_1+a_2+\cdots+a_n| \leq |a_1| + |a_2| + \cdots + |a_n| \text{ for } n \text{ numbers } a_1, a_2, \ldots, a_n."$$

    -   If $n=1$, $P_1$ is true since $|a_1| \leq |a_1|$. In particular,
        $|a_1| = |a_1|$.

    -   Suppose $P_n$ is true. That is, we suppose
        $$|a_1+a_2+\cdots+a_n| \leq |a_1| + |a_2| + \cdots + |a_n|$$ for
        $n$ numbers $a_1,a_2,\ldots,a_n$ is true.

    -   We wish to prove that $P_{n+1}$ holds based on the hypothesis.
        By Triangle Inequality, $$|a_1+a_2+\cdots+a_n + a_{n+1}|$$
        $$= |(a_1+a_2+\cdots+a_n) + a_{n+1}|$$
        $$\leq |a_1+a_2+\cdots+a_n| + |a_{n+1}|$$
        $$\leq |a_1| + |a_2| + \cdots + |a_n| + |a_{n+1}|.$$ Therefore,
        $P_{n+1}$ holds if $P_n$ holds.

    By principle of mathematical induction, we conclude that $P_n$ is
    true for all natural numbers $n$.

#### 4.1

For each set below that is bounded above, list three upper bounds for
the set. Otherwise, write \`\`NOT BOUNDED ABOVE“ or \`\`NBA.”

1.  $(0,1)$ : bounded above. Three upper bounds: $1,2,3$.

2.  $\{\pi,e\}$ : bounded above. Three upper bounds: $\pi,2\pi,3\pi$.

3.  $\{0\}$: bounded above. Three upper bounds: $0,1,2$.

4.  $\displaystyle \bigcup_{n=1}^{\infty}[2n,2n+1]$:\
    $\displaystyle \bigcup_{n=1}^{\infty}[2n,2n+1] = [2,3] \cup [4,5] \cup [6,7] \cup \cdots$\
    NOT BOUNDED ABOVE.

5.  $\{1-\frac{1}{3^n} : n \in {\mathbb{N}}\}$ :\
    $\{1-\frac{1}{3^n} : n \in {\mathbb{N}}\} = \{\frac{2}{3},\frac{8}{9},\frac{26}{27},\frac{80}{81},\ldots\}$.
    Note $\lim_{n\to\infty} 1-\frac{1}{3^n} = 1 - 0 = 1$.\
    Bounded above. Three upper bounds: 1, 2, 3.

6.  $\{r \in {\mathbb{Q}}: r < 2\}$: bounded above. Three upper bounds:
    $2, \frac{5}{2}, 3$.

7.  $\{r \in {\mathbb{Q}}: r^2 < 2\}$ :\
    $\{r \in {\mathbb{Q}}: r^2 < 2\} =\{r \in {\mathbb{Q}}: -\sqrt{2} < r < \sqrt {2}\}$.\
    Bounded above. Three upper bounds:
    $\frac{15}{10},\frac{16}{10},\frac{17}{10}$.

8.  $\{1,\frac{\pi}{3},\pi^2,10\}$ : bounded above. Three upper bounds:
    $10,11,12$.

9.  $\displaystyle \bigcap_{n=1}^{\infty} \left(1-\frac{1}{n}, 1+ \frac{1}{n}\right)$
    :\
    $\displaystyle \bigcap_{n=1}^{\infty} \left(1-\frac{1}{n}, 1+ \frac{1}{n}\right) = (0,2) \cap \left(\frac{1}{2}, \frac{3}{2}\right) \cap \left(\frac{2}{3}, \frac{4}{3}\right) \cap \left(\frac{3}{4}, \frac{5}{4}\right) \cap \left(\frac{4}{5},\frac{6}{5}\right) \cap \cdots$.
    Note
    $\lim_{n\to\infty} \left(1-\frac{1}{n},1+\frac{1}{n}\right) = (1-0,1+0) = (1,1) = \{1\}$.\
    Bounded above. Three upper bounds: $1,2,3$.

10. $\{x \in {\mathbb{R}}: x^3 < 8\}$ :\
    $\{x \in {\mathbb{R}}: x^3 < 8\} = \{x \in {\mathbb{R}}: x < 2\}$.\
    Bounded above. Three upper bounds: $2,3,4$.

11. $\{\cos{\left(\frac{n\pi}{3}\right)} : n \in {\mathbb{N}}\}$ :\
    $$\{\cos{\left(\frac{n\pi}{3}\right)} : n \in {\mathbb{N}}\}$$
    $$= \left\{\cos{\left(\frac{\pi}{3}\right)},
        \cos{\left(\frac{2\pi}{3}\right)},
        \cos{(\pi)},
        \cos{\left(\frac{4\pi}{3}\right)},
        \cos{\left(\frac{5\pi}{3}\right)},
        \cos{(2\pi)}, \cos{\left(\frac{7\pi}{3}\right)}, \ldots \right\}$$
    $$= \left\{\frac{1}{2},-\frac{1}{2},-1,-\frac{1}{2},\frac{1}{2},1, \frac{1}{2}, \ldots \right\}.$$
    Bounded Above. Three upper bounds: $1,2,3$.

#### 4.6

Let $S$ be a nonempty bounded subset of ${\mathbb{R}}$.

1.  Prove $\inf S \leq \sup S$. *Hint:* This is almost obvious; your
    proof should be short.

    Let $s \in S$. Since $\inf S$ is the greatest lower bound of $S$,
    and $\sup S$ is the least upper bound of $S$,
    $$\inf S \leq s \leq \sup S.$$ Thus, by transitivity,
    $\inf S \leq \sup S$.

2.  What can you say about $S$ if $\inf S = \sup S$?\
    \
    Given that $s \in S$, $\inf S \leq s \leq \sup S$, and
    $\inf S = \sup S$, $\inf S = s = \sup S$ must hold. Let’s denote
    $x = \inf S = \sup S$. The set $S$ can only contain an element,
    which is $x$.

#### 4.7

Let $S$ and $T$ be nonempty bounded subsets of ${\mathbb{R}}$.

1.  Prove if $S \subseteq T$, then
    $\inf T \leq \inf S \leq \sup S \leq \sup T$.

    Assume $S \subseteq T$. Let $s \in S$ and $t \in T$. Since $\inf T$
    is the lower bound of $T$ and $\sup T$ is the upper bound of $T$,
    $\inf T \leq t \leq \sup T$. Since $S \subseteq T$, $s \in T$. Thus,
    $\inf T \leq s \leq \sup T$, which means that $\inf T$ is an lower
    bound of $S$ while $\sup T$ is an upper bound of $S$. Since $\inf S$
    is the greatest lower bound of $S$ , $\inf T \leq \inf S$. Since
    $\sup S$ is the least upper bound of $S$, $\sup S \leq \sup T$.
    Therefore, $\inf T \leq \inf S \leq \sup S \leq \sup T$.

2.  Prove $\sup (S \cup T) = \max \{ \sup S,\sup T\}$. *Note:* In part
    (b), do *Note:* In part (b), do *not* assume $S \subseteq T$.

    Since $S \subseteq S \cup T$, $\sup S \leq \sup (S \cup T)$.
    Similarly, since $T \subseteq S \cup T$,
    $\sup T \leq \sup (S \cup T)$. Thus,
    $\max\{\sup S, \sup T\} \leq \sup(S \cup T)$. In order to show that
    $\sup (S \cup T) = \max \{ \sup S,\sup T\}$, we must also show that
    $\sup (S \cup T) \leq \max \{\sup S, \sup T\}$. Assume $x \in S$.
    Then $x \leq \sup S \leq \max\{\sup S, \sup T\}$. Assume $x \in T$.
    Then $x \leq \sup T \leq \max\{\sup S, \sup T\}$. Thus,
    $x \leq \max\{\sup S, \sup T\}$ $\forall x \in S \cup T$. Hence,
    $\max\{\sup S, \sup T\}$ is an upper bound of $S \cup T$, and as a
    result, $\sup (S \cup T) \leq \max\{\sup S, \sup T\}$ for
    $\sup (S \cup T)$ is the least upper bound of $S \cup T$. Since
    $\max \{\sup S, \sup T\} \leq \sup (S \cup T)$ and
    $\sup (S \cup T) \leq \max\{\sup S, \sup T\}$,
    $\sup (S \cup T) = \max \{\sup S, \sup T\}$.

#### 4.8

Let $S$ and $T$ be nonempty subsets of ${\mathbb{R}}$ with the following
property: $s \leq t$ for all $s \in S$ and $t \in T$.

1.  Observe $S$ is bounded above and $T$ is bounded below.\
    \
    As further explanation, since there exists a real number $t$ such
    that $s \leq t$ for all $s \in S$, $S$ is bounded above. Since there
    exists a real number $s$ such that $s \leq t$ for all $t \in T$, $T$
    is bounded below.

2.  Prove $\sup S \leq \inf T$.\
    \
    According to page 22 of Ross’ *Elementary Analysis* (2nd ed.), if
    $S$ is bounded above, then $M = \sup S$ if and only if

    1.  $s \leq M$ for all $s \in S$, and

    2.  whenever $M_1 < M$, there exists $s_1 \in S$ such that
        $s_1 > M_1$.

    Similarly, $m = \inf S$ if and only if

    1.  $s \geq m$ for all $s \in S$, and

    2.  whenever $m_1 > m$, there exists $s_1 \in S$ such that
        $s_1 < m_1$.

    *Proof by Contradiction.* Assume the contrary, $\inf T < \sup S$.
    Thus, by property (ii) of supremum, $\exists s_1 \in S$ such that
    $s_1 > \inf T$, and if $s_1 > \inf T$, $\exists t_1 \in T$ such that
    $\inf T \leq t_1 < s_1$. Thus, $s_1 > t_1$, which contradicts the
    assumption that $s \leq t$. Thus, $\inf T \geq \sup S$.

3.  Give an example of sets $S$ and $T$ where $S \cap T$ is nonempty.\
    \
    Consider $S = [0,2]$ and $T = [2,3]$. Note that $S \cap T = \{2\}$,
    which is nonempty.

4.  Give an example of sets $S$ and $T$ where $\sup S = \inf T$ and
    $S \cap T$ is the empty set.\
    \
    Consider $S = [0,2)$ and $T = (2,3]$. Note that
    $S \cap T = \emptyset$ and that $\sup S = 2$ and $\inf T = 2$. Thus,
    $\sup S = \inf T$.

#### 4.10

Prove that if $a > 0$, then there exists $n \in {\mathbb{N}}$ such that
$\frac{1}{n} < a < n$.

The Archimedean Property states that if $a >0$ and $b>0$, then for
$n \in {\mathbb{N}}$, we have $n a > b$. Given $a > 0$ and $1 >0$, for
$n_1 \in {\mathbb{N}}$, we have $$n_1 a > 1,$$ and as a result,
$$a > \frac{1}{n_1} \text{, or } \frac{1}{n_1} < a.$$ Note that for
$n_2 \in {\mathbb{N}}$, the inequality $$n_2 \cdot 1 > a$$ also applies
with the Archimedean Property. Thus, $$n_2 > a \text{, or } a < n_2.$$
Consider $n = \max \{n_1, n_2\}$. Since
$$a > \frac{1}{n_1} \geq \frac{1}{n}$$ and $$a < n_2 \leq n \text{,}$$
$$\frac{1}{n} < a < n.$$

#### 4.11

Consider $a,b \in {\mathbb{R}}$ where $a < b$. Use Denseness of
${\mathbb{Q}}$ to show there are infinitely many rationals between $a$
and $b$.\
\
*Proof by Induction.* By the Denseness of ${\mathbb{Q}}$,
$\exists r_1 \in {\mathbb{Q}}$ such that $a < r_1 < b$. Similarly, by
the Denseness of ${\mathbb{Q}}$, $\exists r_2 \in {\mathbb{Q}}$ such
that $a < r_2 < r_1$. If we continue, we have
$a < r_n < r_{n-1} < \cdots r_2 < r_1 < b$ where $n$ is the times we use
Denseness of ${\mathbb{Q}}$. Given $n \in {\mathbb{N}}$, assume
$\exists r_n \in {\mathbb{Q}}$ such that $a < r_n < b$. Then, by the
Denseness of ${\mathbb{Q}}$, $\exists r_{n+1} \in {\mathbb{Q}}$ such
that $a < r_{n+1} < r_n$. Thus, by the principle of induction, there are
infinitely many rationals between $a$ and $b$ given
$a,b \in {\mathbb{R}}$. In other words,
$\exists r_1, r_2, \ldots \in (a,b) \cap {\mathbb{Q}}$.

#### 4.12

Let ${\mathbb{I}}$ be the set of real numbers that are not rational;
elements of ${\mathbb{I}}$ are called *irrational numbers*. Prove if
$a < b$, then there exists $x \in {\mathbb{I}}$ such that $a < x < b$.
*Hint*: First show
$\{r+\sqrt{2} : r \in {\mathbb{Q}}\} \subseteq {\mathbb{I}}$.

#### 4.14

Let $A$ and $B$ be nonempty bounded subsets of ${\mathbb{R}}$, and let
$A + B$ be the set of all sums $a+b$ where $a \in A$ and $b \in B$.

1.  Prove $\sup (A+B) = \sup A + \sup B$. *Hint:* To show
    $\sup A + \sup B \leq \sup (A+B)$, show that for each $b \in B$,
    $\sup (A+B)-b$ is an upper bound for $A$, hence
    $\sup A \leq \sup (A+B)-b$. Then show $\sup (A+B) - \sup A$ is an
    upper bound for $B$.

    Given that $A$ and $B$ are bounded, $A$ and $B$ both have least
    upper bounds as shown in the following.

    -   $a \leq \sup A$ $\forall a \in A$

    -   $b \leq \sup B$ $\forall b \in B$

    Let $x \in (A+B)$, then $x = a+b$ for some $a \in A$ and $b \in B$.
    Note that $$a+b \leq \sup A + b \leq \sup A + \sup B.$$ Thus,
    $(A+B)$ is bounded above since
    $$x \leq \sup A + \sup B \text{ for } x \in (A+B).$$ With
    $\sup A + \sup B$ being the upper bound of $(A+B)$ and $\sup (A+B)$
    being the least upper bound of $(A+B)$,
    $$\sup (A+B) \leq \sup A + \sup B.$$ Now to show that
    $\sup A + \sup B \leq \sup (A+B)$, we first need to show that for
    each $b \in B$, $\sup (A+B) - b$ is an upper bound for $A$. Since
    $\sup (A+B)$ is the least upper bound of $(A+B)$,
    $$a+b \leq \sup (A+B) \text{ for } a+b \in (A+B),$$ which implies
    that $$a \leq \sup (A+B) -b \text{ for } a \in A.$$ Thus,
    $\sup (A+B) - b$ is an upper bound of $A$. With $\sup A$ being the
    least upper bound of $A$, we have $$\sup A \leq \sup (A+B) - b.$$ If
    we apply algebraic manipulation to the inequality, we have
    $b \leq \sup (A+B) - \sup A$ for $b \in B$ as shown below.
    $$\sup A \leq \sup (A+B) - b$$ $$\sup A + b \leq \sup (A+B)$$
    $$b \leq \sup (A+B) - \sup A$$ Thus, $\sup (A+B) - \sup A$ is an
    upper bound for $B$. With $\sup B$ being the least upper bound for
    $B$, we have $$\sup B \leq \sup (A+B) - \sup A.$$ By adding $\sup A$
    to both sides of the inequality, we have
    $$\sup A + \sup B \leq \sup (A+B).$$ Since
    $\sup (A+B) \leq \sup A + \sup B$ and
    $\sup A + \sup B \leq \sup (A+B)$, $$\sup (A+B) = \sup A + \sup B.$$

2.  Prove $\inf (A+B) = \inf A + \inf B$.

    Given that $A$ and $B$ are bounded, $A$ and $B$ both have greatest
    lower bounds as shown in the following.

    -   $a \geq \inf A$ $\forall a \in A$

    -   $b \geq \inf B$ $\forall b \in B$

    Let $x \in (A+B)$, then $x = a+b$ for some $a \in A$ and $b \in B$.
    Note that $$a+b \geq \inf A + b \geq \inf A + \inf B.$$ Thus,
    $(A+B)$ is bounded below since
    $$x \geq \inf A + \inf B \text{ for } x \in (A+B).$$ With
    $\inf A + \inf B$ being the lower bound of $(A+B)$ and $\inf (A+B)$
    being the greatest lower bound of $(A+B)$,
    $$\inf (A+B) \geq \inf A + \inf B.$$ Now to show that
    $\inf (A+B) \leq \inf A + \inf B$, we need to first show that for
    each $b \in B$, $\inf (A+B) - b$ is a lower bound for $A$. Since
    $\inf (A+B)$ is the greatest lower bound of $(A+B)$,
    $$a+b \geq \inf (A+B) \text{ for } a+b \in (A+B),$$ which implies
    that $$a \geq \inf (A+B) - b \text{ for } a \in A.$$ Thus,
    $\inf (A+B) - b$ is a lower bound of $A$. With $\inf A$ being the
    greatest lower bound of $A$, we have $$\inf A \geq \inf (A+B) - b.$$
    If we apply algebraic manipulation to the inequality, we have
    $b \geq \inf (A+B) - \inf A$ for $b \in B$ as shown below.
    $$\inf A \geq \inf (A+B) - b$$ $$\inf A + b \geq \inf (A+B)$$
    $$b \geq \inf (A+B) - \inf A$$ Thus, $\inf (A+B) - \inf A$ is a
    lower bound for $B$. With $\inf B$ being the greatest lower bound
    for $B$, we have $$\inf B \geq \inf (A+B) - \inf A.$$ By adding
    $\inf A$ to both sides of the inequality, we have
    $$\inf A + \inf B \geq \inf(A+B).$$ Since
    $\inf (A+B) \geq \inf A + \inf B$ and
    $\inf A + \inf B \geq \inf (A+B)$, $$\inf (A+B) = \inf A + \inf B.$$

#### 4.15

Let $a,b \in {\mathbb{R}}$. Show if $a \leq b + \frac{1}{n}$ for all
$n \in {\mathbb{N}}$, then $a \leq b$. Compare Exercise 3.8.\
\
*Proof by Contradiction.* Let $a,b \in {\mathbb{R}}$, and
$a \leq b + \frac{1}{n}$ for all $n \in {\mathbb{N}}$. We would like to
show that $a \leq b$. Assume the contrary, $a>b$. Then $a-b > 0$. Since
$a-b>0$ and $1>0$, by the Archimedian Property,
$\exists n_0 \in {\mathbb{N}}$ such that $n_0 (a-b) > 1 $. If we
algebraically manipulate the inequality, $a > b + \frac{1}{n_0}$ as
shown below. $$n_0 (a-b) > 1$$ $$a-b > \frac{1}{n_0}$$
$$a > b + \frac{1}{n_0}$$ Thus, by contradiction, $a \leq b$ given that
$a \leq b + \frac{1}{n}$ for all $n \in {\mathbb{N}}$.

#### 5.2

Give the infimum and supremum of each set listed in Exercise 5.1.

1.  $\{x \in {\mathbb{R}}: x < 0\}$

    -   $\inf \{x \in {\mathbb{R}}: x < 0\} = -\infty$

    -   $\sup \{x \in {\mathbb{R}}: x < 0\} = 0$

2.  $\{x \in {\mathbb{R}}: x^3 \leq 8\}$
    $$\{x \in {\mathbb{R}}: x^3 \leq 8\} = \{x \in {\mathbb{R}}: x \leq 2\}$$

    -   $\inf \{x \in {\mathbb{R}}: x^3 \leq 8\} = -\infty$

    -   $\sup \{x \in {\mathbb{R}}: x^3 \leq 8\} = 2$

3.  $\{x^2 : x \in {\mathbb{R}}\}$
    $$\{x^2 : x \in {\mathbb{R}}\} = \{\sqrt{x} : x \in {\mathbb{R}}\}$$

    -   Since $\sqrt{x} > 0$, $\inf \{x^2 : x \in {\mathbb{R}}\} = 0$.

    -   Since $\displaystyle \lim_{x \to \infty} \sqrt{x} = \infty$,
        $\sup \{x^2 : x \in {\mathbb{R}}\} = \infty$.

4.  $\{x \in {\mathbb{R}}: x^2 < 8\}$
    $$\{x \in {\mathbb{R}}: x^2 < 8\} = \{x \in {\mathbb{R}}: x < 2\sqrt{2}\}$$

    -   $\inf \{x \in {\mathbb{R}}: x^2 < 8\} = -2 \sqrt{2}$

    -   $\sup \{x \in {\mathbb{R}}: x^2 < 8\} = 2 \sqrt{2}$


